refactor delim

theories/examples/delim_lang/lang.v
@@ -1,10 +1,7 @@
 From gitrees Require Export prelude.
 From stdpp Require Import gmap.
-(* From iris.heap_lang Require Import locations. *)
 Require Import Binding.Resolver Binding.Lib Binding.Set Binding.Auto Binding.Env.
 
-(* Definition loc : Set := locations.loc. *)
-(* Global Instance loc_dec_eq (l l' : loc) : Decision (l = l') := _. *)
 Variant nat_op := Add | Sub | Mult.
 
 Inductive expr {X : Set} :=
@@ -21,15 +18,10 @@ Inductive expr {X : Set} :=
 (* The effects *)
 | Shift (e : @expr (inc X)) : expr
 | Reset (e : expr) : expr
-(* | Alloc (e : expr) : expr *)
-(* | Deref (e : expr) : expr *)
-(* | Assign (e₁ : expr) (e₂ : expr) : expr *)
 with val {X : Set} :=
 | LitV (n : nat) : val
 | RecV (e : @expr (inc (inc X))) : val
 | ContV (k : cont) : val
-(* | LocV (l : loc) : val *)
-(* | UnitV : val *)
 with cont {X : Set} :=
 | END : cont
 | IfK (e1 : expr) (e2 : expr) : cont -> cont
@@ -39,10 +31,6 @@ with cont {X : Set} :=
 | AppContRK (e : expr) : cont -> cont (* e ◻ *)
 | NatOpLK (op : nat_op) (v : val) : cont -> cont (* ◻ + v *)
 | NatOpRK (op : nat_op) (e : expr) : cont -> cont (* e + ◻ *)
-(* | AllocK : cont → cont *)
-(* | DerefK : cont → cont *)
-(* | AssignRK (e : expr) : cont → cont (* E <- e *) *)
-(* | AssignLK (v : val) : cont → cont (* v <- E *) *)
 .
 (* conts are inside-out contexts: eg
  IfK e1 e2 (AppLK v ◻) ==> App (if ◻ then e1 else e2) v*)
@@ -63,9 +51,6 @@ Fixpoint emap {A B : Set} (f : A [→] B) (e : expr A) : expr B :=
   | If e₁ e₂ e₃ => If (emap f e₁) (emap f e₂) (emap f e₃)
   | Shift e => Shift (emap (f ↑) e)
   | Reset e => Reset (emap f e)
-  (* | Alloc e => Alloc (emap f e) *)
-  (* | Deref e => Deref (emap f e) *)
-  (* | Assign e₁ e₂ => Assign (emap f e₁) (emap f e₂) *)
   end
 with
 vmap {A B : Set} (f : A [→] B) (v : val A) : val B :=
@@ -73,8 +58,6 @@ vmap {A B : Set} (f : A [→] B) (v : val A) : val B :=
   | LitV n => LitV n
   | RecV e => RecV (emap ((f ↑) ↑) e)
   | ContV k => ContV (kmap f k)
-  (* | LocV l => LocV l *)
-  (* | UnitV => UnitV *)
   end
 with kmap {A B : Set} (f : A [→] B) (K : cont A) : cont B :=
    match K with
@@ -86,10 +69,6 @@ with kmap {A B : Set} (f : A [→] B) (K : cont A) : cont B :=
    | AppContRK e k => AppContRK (emap f e) (kmap f k)
    | NatOpLK op v k => NatOpLK op (vmap f v) (kmap f k)
    | NatOpRK op e k => NatOpRK op (emap f e) (kmap f k)
-   (* | AllocK k => AllocK (kmap f k) *)
-   (* | DerefK k => DerefK (kmap f k) *)
-   (* | AssignRK e k => AssignRK (emap f e) (kmap f k) *)
-   (* | AssignLK v k => AssignLK (vmap f v) (kmap f k) *)
    end.
 
 
@@ -109,9 +88,6 @@ Fixpoint ebind {A B : Set} (f : A [⇒] B) (e : expr A) : expr B :=
   | If e₁ e₂ e₃ => If (ebind f e₁) (ebind f e₂) (ebind f e₃)
   | Shift e => Shift (ebind (f ↑) e)
   | Reset e => Reset (ebind f e)
-  (* | Alloc e => Alloc (ebind f e) *)
-  (* | Deref e => Deref (ebind f e) *)
-  (* | Assign e₁ e₂ => Assign (ebind f e₁) (ebind f e₂) *)
   end
 with
 vbind {A B : Set} (f : A [⇒] B) (v : val A) : val B :=
@@ -119,8 +95,6 @@ vbind {A B : Set} (f : A [⇒] B) (v : val A) : val B :=
   | LitV n => LitV n
   | RecV e => RecV (ebind ((f ↑) ↑) e)
   | ContV k => ContV (kbind f k)
-  (* | LocV l => LocV l *)
-  (* | UnitV => UnitV *)
   end
 with kbind {A B : Set} (f : A [⇒] B) (K : cont A) : cont B :=
    match K with
@@ -132,10 +106,6 @@ with kbind {A B : Set} (f : A [⇒] B) (K : cont A) : cont B :=
    | AppContRK e k => AppContRK (ebind f e) (kbind f k)
    | NatOpLK op v k => NatOpLK op (vbind f v) (kbind f k)
    | NatOpRK op e k => NatOpRK op (ebind f e) (kbind f k)
-   (* | AllocK k => AllocK (kbind f k) *)
-   (* | DerefK k => DerefK (kbind f k) *)
-   (* | AssignRK e k => AssignRK (ebind f e) (kbind f k) *)
-   (* | AssignLK v k => AssignLK (vbind f v) (kbind f k) *)
    end.
 
 #[export] Instance BindCore_expr : BindCore expr := @ebind.
@@ -315,10 +285,6 @@ Fixpoint fill {X : Set} (K : cont X) (e : expr X) : expr X :=
   | AppContRK el K => fill K (AppCont el e)
   | NatOpLK op v K => fill K (NatOp op e (Val v))
   | NatOpRK op el K => fill K (NatOp op el e)
-  (* | AllocK K => fill K (Alloc e) *)
-  (* | DerefK K => fill K (Deref e) *)
-  (* | AssignRK e' K => fill K (Assign e e') *)
-  (* | AssignLK v K => fill K (Assign (Val v) e) *)
   end.
 
 (*** Continuation operations *)
@@ -345,10 +311,6 @@ Fixpoint cont_compose {S} (K1 K2 : cont S) : cont S :=
   | AppContRK e K => AppContRK e (cont_compose K1 K)
   | NatOpLK op v K => NatOpLK op v (cont_compose K1 K)
   | NatOpRK op e K => NatOpRK op e (cont_compose K1 K)
-  (* | AllocK K => AllocK (cont_compose K1 K) *)
-  (* | DerefK K => DerefK (cont_compose K1 K) *)
-  (* | AssignRK e' K => AssignRK e' (cont_compose K1 K) *)
-  (* | AssignLK v K => AssignLK v (cont_compose K1 K) *)
   end.
 
 Lemma fill_comp {S} (K1 K2 : cont S) e : fill (cont_compose K1 K2) e = fill K1 (fill K2 e).
@@ -366,7 +328,6 @@ Qed.
 (*** Abstract Machine semantics *)
 
 Definition Mcont {S} := list $ cont S.
-(* Definition state X := gmap loc (val X). *)
 
 Variant config {S} : Type :=
   | Ceval : expr S -> cont S -> @Mcont S → config
@@ -378,108 +339,80 @@ Variant config {S} : Type :=
 Reserved Notation "c '===>' c' / nm"
   (at level 40, c', nm at level 30).
 
-Variant Cred {S : Set} : config (* * state S *) -> config (* * state S *)
-                         -> (nat * nat) -> Prop :=
+Variant Cred {S : Set} : config -> config -> (nat * nat) -> Prop :=
 (* init *)
-| Ceval_init : forall (e : expr S) (* σ *),
-  (Cexpr e(* , σ *)) ===> (Ceval e END [](* , σ *)) / (0,0)
+| Ceval_init : forall (e : expr S),
+  (Cexpr e) ===> (Ceval e END []) / (0,0)
 
 (* eval *)
-| Ceval_val : forall v k mk (* σ *),
-  (Ceval (Val v) k mk(* , σ *)) ===> (Ccont k v mk(* , σ *)) / (0,0)
+| Ceval_val : forall v k mk,
+  (Ceval (Val v) k mk) ===> (Ccont k v mk) / (0,0)
 
-| Ceval_app : forall e0 e1 k mk (* σ *),
-  (Ceval (App e0 e1) k mk(* , σ *)) ===> (Ceval e0 (AppLK e1 k) mk(* , σ *)) / (0,0)
+| Ceval_app : forall e0 e1 k mk,
+  (Ceval (App e0 e1) k mk) ===> (Ceval e0 (AppLK e1 k) mk) / (0,0)
 
-| Ceval_app_cont : forall e0 e1 k mk (* σ *),
-  (Ceval (AppCont e0 e1) k mk(* , σ *)) ===> (Ceval e1 (AppContRK e0 k) mk(* , σ *)) / (0,0)
+| Ceval_app_cont : forall e0 e1 k mk,
+  (Ceval (AppCont e0 e1) k mk) ===> (Ceval e1 (AppContRK e0 k) mk) / (0,0)
 
-| Ceval_natop : forall op e0 e1 k mk (* σ *),
-  (Ceval (NatOp op e0 e1) k mk(* , σ *)) ===> (Ceval e1 (NatOpRK op e0 k) mk(* , σ *)) / (0,0)
+| Ceval_natop : forall op e0 e1 k mk,
+  (Ceval (NatOp op e0 e1) k mk) ===> (Ceval e1 (NatOpRK op e0 k) mk) / (0,0)
 
-| Ceval_if : forall eb et ef k mk (* σ *),
-  (Ceval (If eb et ef) k mk(* , σ *)) ===> (Ceval eb (IfK et ef k) mk(* , σ *)) / (0,0)
+| Ceval_if : forall eb et ef k mk,
+  (Ceval (If eb et ef) k mk) ===> (Ceval eb (IfK et ef k) mk) / (0,0)
 
-| Ceval_reset : forall e k mk (* σ *),
-  (Ceval (Reset e) k mk(* , σ *)) ===> (Ceval e END (k :: mk)(* , σ *)) / (1, 1)
+| Ceval_reset : forall e k mk,
+  (Ceval (Reset e) k mk) ===> (Ceval e END (k :: mk)) / (1, 1)
 
-| Ceval_shift : forall (e : expr $ inc S) k mk (* σ *),
-  (Ceval (Shift e) k mk(* , σ *)) ===>
-    (Ceval (subst (Inc := inc) e (Val $ ContV k)) END mk(* , σ *)) / (1, 1)
+| Ceval_shift : forall (e : expr $ inc S) k mk,
+  (Ceval (Shift e) k mk) ===>
+    (Ceval (subst (Inc := inc) e (Val $ ContV k)) END mk) / (1, 1)
 
 (* cont *)
-| Ccont_end : forall v mk (* σ *),
-  (Ccont END v mk(* , σ *)) ===> (Cmcont mk v(* , σ *)) / (0,0)
+| Ccont_end : forall v mk,
+  (Ccont END v mk) ===> (Cmcont mk v) / (0,0)
 
-| Ccont_appl : forall e v k mk (* σ *),
-  (Ccont (AppLK e k) v mk(* , σ *)) ===> (Ceval e (AppRK v k) mk(* , σ *)) / (0, 0)
+| Ccont_appl : forall e v k mk,
+  (Ccont (AppLK e k) v mk) ===> (Ceval e (AppRK v k) mk) / (0, 0)
 
-| Ccont_app_contr : forall e v k mk (* σ *),
-  (Ccont (AppContRK e k) v mk(* , σ *)) ===> (Ceval e (AppContLK v k) mk(* , σ *)) / (0, 0)
+| Ccont_app_contr : forall e v k mk,
+  (Ccont (AppContRK e k) v mk) ===> (Ceval e (AppContLK v k) mk) / (0, 0)
 
-| Ccont_appr : forall e v k mk (* σ *),
-  (Ccont (AppRK (RecV e) k) v mk(* , σ *)) ===>
+| Ccont_appr : forall e v k mk,
+  (Ccont (AppRK (RecV e) k) v mk) ===>
     (Ceval (subst (Inc := inc)
               (subst (F := expr) (Inc := inc) e
                  (Val (shift (Inc := inc) v)))
-              (Val (RecV e))) k mk(* , σ *)) / (1, 0)
+              (Val (RecV e))) k mk) / (1, 0)
 
-| Ccont_cont : forall v k k' mk (* σ *),
-  (Ccont (AppContLK v k) (ContV k') mk(* , σ *)) ===>
-    (Ccont k' v (k :: mk)(* , σ *)) / (2, 1)
+| Ccont_cont : forall v k k' mk,
+  (Ccont (AppContLK v k) (ContV k') mk) ===>
+    (Ccont k' v (k :: mk)) / (2, 1)
 
-| Ccont_if : forall et ef n k mk (* σ *),
-  (Ccont (IfK et ef k) (LitV n) mk(* , σ *)) ===>
-    (Ceval (if (n =? 0) then ef else et) k mk(* , σ *)) / (0, 0)
+| Ccont_if : forall et ef n k mk,
+  (Ccont (IfK et ef k) (LitV n) mk) ===>
+    (Ceval (if (n =? 0) then ef else et) k mk) / (0, 0)
 
-| Ccont_natopr : forall op e v k mk (* σ *),
-  (Ccont (NatOpRK op e k) v mk(* , σ *)) ===>
-    (Ceval e (NatOpLK op v k) mk(* , σ *)) / (0, 0)
+| Ccont_natopr : forall op e v k mk,
+  (Ccont (NatOpRK op e k) v mk) ===>
+    (Ceval e (NatOpLK op v k) mk) / (0, 0)
 
-| Ccont_natopl : forall op v0 v1 v2 k mk (* σ *),
+| Ccont_natopl : forall op v0 v1 v2 k mk,
   nat_op_interp op v0 v1 = Some v2 ->
-  (Ccont (NatOpLK op v1 k) v0 mk(* , σ *)) ===>
-    (Ceval (Val v2) k mk(* , σ *)) / (0,0)
+  (Ccont (NatOpLK op v1 k) v0 mk) ===>
+    (Ceval (Val v2) k mk) / (0,0)
 
 (* meta-cont *)
-| Cmcont_cont : forall k mk v (* σ *),
-  (Cmcont (k :: mk) v(* , σ *)) ===> (Ccont k v mk(* , σ *)) / (1,1)
+| Cmcont_cont : forall k mk v,
+  (Cmcont (k :: mk) v) ===> (Ccont k v mk) / (1,1)
 
-| Cmcont_ret : forall v (* σ *),
-  (Cmcont [] v(* , σ *)) ===> (Cret v(* , σ *)) / (1, 1)
-
-(* | Ceval_assign : forall e0 e1 k mk σ, *)
-(*   (Ceval (Assign e0 e1) k mk, σ) ===> (Ceval e1 (AssignRK e0 k) mk, σ) / (0, 0) *)
-
-(* | Ccont_assignr : forall e v k mk σ, *)
-(*   (Ccont (AssignRK e k) v mk, σ) ===> (Ceval e (AssignLK v k) mk, σ) / (0, 0) *)
-
-(* | Ccont_assignl : forall l v' k mk σ, *)
-(*   (Ccont (AssignLK (LocV l) k) v' mk, σ) ===> *)
-(*     (Ceval (Val UnitV) k mk, <[l:=v']>σ) / (0, 1) *)
-
-(* | Ceval_alloc : forall e k mk σ, *)
-(*   (Ceval (Alloc e) k mk, σ) ===> (Ceval e (AllocK k) mk, σ) / (0, 0) *)
-
-(* | Ceval_allock : ∀ l v k mk σ, *)
-(*   σ !! l = None -> *)
-(*   (Ccont (AllocK k) v mk, σ) ===> *)
-(*     (Ceval (Val (LocV l)) k mk, <[l:=v]>σ) / (0, 1) *)
-
-(* | Ceval_deref : forall e k mk σ, *)
-(*   (Ceval (Deref e) k mk, σ) ===> (Ceval e (DerefK k) mk, σ) / (0, 0) *)
-
-(* | Ceval_derefk : ∀ l v k mk σ, *)
-(*   σ !! l = Some v -> *)
-(*   (Ccont (DerefK k) (LocV l) mk, σ) ===> *)
-(*     (Ceval (Val v) k mk, σ) / (0, 1) *)
+| Cmcont_ret : forall v,
+  (Cmcont [] v) ===> (Cret v) / (1, 1)
 where "c ===> c' / nm" := (Cred c c' nm).
 
 Arguments Mcont S%bind : clear implicits.
 Arguments config S%bind : clear implicits.
 
-Inductive steps {S} : config S (* * state S *) -> config S (* * state S *) ->
-                      (nat * nat) -> Prop :=
+Inductive steps {S} : config S -> config S -> (nat * nat) -> Prop :=
 | steps_zero : forall c,
   steps c c (0, 0)
 | steps_many : forall c1 c2 c3 n m n' m' n'' m'',
@@ -512,6 +445,43 @@ Proof.
   - apply G.
 Qed.
 
+Lemma step_pack {S : Set} (a b : config S) :
+  ∀ nm, Cred a b nm → stepEx a b.
+Proof.
+  intros nm H.
+  by exists nm.
+Qed.
+
+Lemma steps_pack {S : Set} (a b : config S) :
+  ∀ nm, steps a b nm → stepsEx a b.
+Proof.
+  intros nm H.
+  by exists nm.
+Qed.
+
+Lemma step_det {S : Set} (c c' c'' : config S)
+  : stepEx c c' → stepEx c c'' → c' = c''.
+Proof.
+  intros [nm H].
+  revert c''.
+  inversion H; subst; intros c'' [nm' G];
+    inversion G; subst; simplify_eq; reflexivity.
+Qed.
+
+Lemma steps_det_val {S : Set} (c c' : config S) (v : val S)
+  : stepsEx c (Cret v) → stepEx c c' → stepsEx c' (Cret v).
+Proof.
+  intros [n H].
+  revert c'.
+  inversion H; subst; intros c' G.
+  - destruct G as [? G].
+    inversion G.
+  - erewrite (step_det c c' c2).
+    + by eapply steps_pack.
+    + assumption.
+    + by eapply step_pack.
+Qed.
+
 Definition meta_fill {S} (mk : Mcont S) e :=
   fold_left (λ e k, fill k e) mk e.
 
@@ -522,7 +492,6 @@ Coercion Val : val >-> expr.
 Declare Scope syn_scope.
 Delimit Scope syn_scope with syn.
 
-(* Coercion LocV : loc >-> val. *)
 Coercion App : expr >-> Funclass.
 
 Class AsSynExpr (F : Set -> Type) := { __asSynExpr : ∀ S, F S -> expr S }.
@@ -606,45 +575,6 @@ Global Instance AppContNotationRK {S : Set} {F : Set -> Type} `{AsSynExpr F} :
   __app_cont e K := cont_compose K (AppContRK (__asSynExpr e) END)
   }.
 
-(* Class AllocNotation (A B : Type) := { __alloc : A -> B }. *)
-(* Notation "'alloc' e" := (__alloc e%syn) (at level 61) : syn_scope. *)
-
-(* Global Instance AllocNotationExpr {S : Set} {F : Set -> Type} `{AsSynExpr F} : *)
-(*   AllocNotation (F S) (expr S) := { __alloc e := Alloc (__asSynExpr e) }. *)
-
-(* Global Instance AllocNotationK {S : Set} : AllocNotation (cont S) (cont S) := *)
-(*   { __alloc K := AllocK K }. *)
-
-(* Class DerefNotation (A B : Type) := { __deref : A -> B }. *)
-(* Notation "'!' e" := (__deref e%syn) (at level 61) : syn_scope. *)
-
-(* Global Instance DerefNotationExpr {S : Set} {F : Set -> Type} `{AsSynExpr F} : *)
-(*   DerefNotation (F S) (expr S) := { __deref e := Deref (__asSynExpr e) }. *)
-
-(* Global Instance DerefNotationK {S : Set} : DerefNotation (cont S) (cont S) := *)
-(*   { __deref K := DerefK K }. *)
-
-(* Class AssignNotation (A B C : Type) := { __assign : A -> B -> C }. *)
-(* (* <- !!! *) *)
-(* Notation "x '<-' y" := (__assign x%syn y%syn) *)
-(*                         (at level 40, y at next level, left associativity) *)
-(*     : syn_scope. *)
-
-(* Global Instance AssignNotationExpr {S : Set} {F G : Set -> Type} *)
-(*   `{AsSynExpr F, AsSynExpr G} : AssignNotation (F S) (G S) (expr S) := { *)
-(*   __assign e₁ e₂ := Assign (__asSynExpr e₁) (__asSynExpr e₂) *)
-(*   }. *)
-
-(* Global Instance AssignNotationLK {S : Set} *)
-(*   : AssignNotation (cont S) (val S) (cont S) := { *)
-(*     __assign K v := AssignLK v K *)
-(*   }. *)
-
-(* Global Instance AssignNotationRK {S : Set} {F : Set -> Type} `{AsSynExpr F} *)
-(*   : AssignNotation (F S) (cont S) (cont S) := { *)
-(*     __assign e K := AssignRK (__asSynExpr e) K *)
-(*   }. *)
-
 Notation of_val := Val (only parsing).
 
 Notation "x '⋆' y" := (__app x%syn y%syn) (at level 40, y at next level
@@ -663,7 +593,6 @@ Notation "'$' fn" := (set_pure_resolver fn) (at level 60) : syn_scope.
 Notation "K '⟪' e '⟫'" := (fill K%syn e%syn) (at level 60) : syn_scope.
 
 Module SynExamples.
-
   Open Scope syn_scope.
 
   Example test1 : expr (inc ∅) := $0.
@@ -671,38 +600,6 @@ Module SynExamples.
   Example test3 : expr ∅ := (rec (reset (shift/cc (($0) @k $1)))).
   Example test4 : expr ∅ :=
     (rec (if ($0) then #1 else (($0) ⋆ (($0) - #1)))).
-  (* Example test5 : expr ∅ := *)
-  (*   ((alloc #1) <- #2). *)
-  (* Example test6 : expr ∅ := *)
-  (*   (! alloc #1). *)
-  (* Example test7 : *)
-  (*   (∃ (ℓ : loc), *)
-  (*      steps (Cexpr (! alloc #1), empty) (Cret (#1 : val ∅), <[ℓ:=#1]>∅%stdpp) (1, 3)). *)
-  (* Proof. *)
-  (*   set (ℓ := (fresh (dom (∅%stdpp : state ∅)))). *)
-  (*   exists ℓ. *)
-  (*   eapply steps_many with _ 0 0 1 3; first reflexivity; first reflexivity; *)
-  (*     first apply Ceval_init. *)
-  (*   eapply steps_many with _ _ _ 1 3; [| | apply Ceval_deref |]; *)
-  (*     first reflexivity; first reflexivity. *)
-  (*   eapply steps_many with _ _ _ 1 3; [| | apply Ceval_alloc |]; *)
-  (*     first reflexivity; first reflexivity. *)
-  (*   eapply steps_many with _ _ _ 1 3; [| | apply Ceval_val |]; *)
-  (*     first reflexivity; first reflexivity. *)
-  (*   eapply steps_many with _ _ _ 1 2; [| | apply (Ceval_allock ℓ) |]; *)
-  (*     first reflexivity; first reflexivity; first set_solver. *)
-  (*   eapply steps_many with _ _ _ 1 2; [| | apply Ceval_val |]; *)
-  (*     first reflexivity; first reflexivity. *)
-  (*   eapply steps_many with _ _ _ 1 _; [| | eapply (Ceval_derefk ℓ (LitV 1)) |]; *)
-  (*     first reflexivity; first reflexivity; first set_solver. *)
-  (*   eapply steps_many with _ _ _ 1 1; [| | apply Ceval_val |]; *)
-  (*     first reflexivity; first reflexivity. *)
-  (*   eapply steps_many with _ _ _ 1 1; [| | apply Ccont_end |]; *)
-  (*     first reflexivity; first reflexivity. *)
-  (*   eapply steps_many with _ _ _ 0 0; [| | apply Cmcont_ret |]; *)
-  (*     first reflexivity; first reflexivity. *)
-  (*   apply steps_zero. *)
-  (* Qed. *)
   Example test8 : expr (inc ∅) := ($ 0).
   Example test9 : val ∅ := (rec (if ($ 1) then # 1 else # 0)).
   Example test10 : expr ∅ := (shift/cc (rec ($ 0))).
