theories/examples/delim_lang/hom.v
@@ -1,0 +1,111 @@
+From gitrees Require Import gitree lang_generic hom.
+From gitrees.effects Require Import delim.
+From gitrees.examples.delim_lang Require Import lang interp.
+
+Require Import Binding.Lib Binding.Set Binding.Env.
+
+Open Scope stdpp_scope.
+
+Section hom.
+  Context {sz : nat}.
+  Context {rs : gReifiers CtxDep sz}.
+  Context {R} `{!Cofe R}.
+  Context `{!SubOfe natO R}.
+  Context `{!subReifier reify_delim rs}.
+  Notation F := (gReifiers_ops rs).
+  Notation IT := (IT F R).
+  Notation ITV := (ITV F R).
+
+  Program Definition AppContRSCtx_HOM {S : Set}
+    (α : @interp_scope F R _ S -n> IT)
+    (env : @interp_scope F R _ S)
+    : HOM := exist _ (interp_app_contrk rs α (λne env, idfun) env) _.
+  Next Obligation.
+    intros; simpl.
+    apply _.
+  Qed.
+
+  Program Definition AppContLSCtx_HOM {S : Set}
+    (β : IT) (env : @interp_scope F R _ S)
+    (Hv : AsVal β)
+    : HOM := exist _ (interp_app_contlk rs (constO β) (λne env, idfun) env) _.
+  Next Obligation.
+    intros; simpl.
+    simple refine (IT_HOM _ _ _ _ _); intros; simpl.
+    - intros ???.
+      do 2 f_equiv.
+      intros ?; simpl.
+      solve_proper.
+    - rewrite get_val_ITV.
+      rewrite get_val_ITV.
+      simpl.
+      rewrite get_fun_tick.
+      reflexivity.
+    - rewrite get_val_ITV.
+      simpl. rewrite get_fun_vis. simpl.
+      f_equiv.
+      intros ?; simpl.
+      apply later_map_ext.
+      intros ?; simpl.
+      rewrite get_val_ITV.
+      simpl.
+      reflexivity.
+    - rewrite get_val_ITV. simpl. rewrite get_fun_err. reflexivity.
+  Qed.
+
+  Program Definition NatOpRSCtx_HOM {S : Set} (op : nat_op)
+    (α : @interp_scope F R _ S -n> IT) (env : @interp_scope F R _ S)
+    : HOM := exist _ (interp_natoprk rs op α (λne env, idfun) env) _.
+  Next Obligation.
+    intros; simpl.
+    apply _.
+  Qed.
+
+  Program Definition NatOpLSCtx_HOM {S : Set} (op : nat_op)
+    (α : IT) (env : @interp_scope F R _ S)
+    (Hv : AsVal α)
+    : HOM := exist _ (interp_natoplk rs op (constO α) (λne env, idfun) env) _.
+  Next Obligation.
+    intros; simpl.
+    apply _.
+  Qed.
+
+  Program Definition AppLSCtx_HOM {S : Set}
+    (α : @interp_scope F R _ S -n> IT)
+    (env : @interp_scope F R _ S)
+    : HOM := exist _ (interp_applk rs α (λne env, idfun) env) _.
+  Next Obligation.
+    intros; simpl.
+    apply _.
+  Qed.
+
+  Transparent LET.
+  Program Definition AppRSCtx_HOM {S : Set}
+    (β : IT) (env : @interp_scope F R _ S)
+    (Hv : AsVal β)
+    : HOM := exist _ (interp_apprk rs (constO β) (λne env, idfun) env) _.
+  Next Obligation.
+    intros; simpl.
+    simple refine (IT_HOM _ _ _ _ _); intros; simpl.
+    - solve_proper_please.
+    - rewrite get_val_ITV.
+      simpl.
+      rewrite get_val_ITV.
+      simpl.
+      rewrite get_val_tick.
+      reflexivity.
+    - rewrite get_val_ITV.
+      simpl.
+      rewrite get_val_vis.
+      do 3 f_equiv.
+      intro; simpl.
+      rewrite get_val_ITV.
+      simpl.
+      reflexivity.
+    - rewrite get_val_ITV.
+      simpl.
+      rewrite get_val_err.
+      reflexivity.
+  Qed.
+  Opaque LET.
+End hom.
