theories/examples/delim_lang/typing.v
@@ -1,0 +1,95 @@
+From gitrees.examples.delim_lang Require Import lang.
+
+Require Import Binding.Lib Binding.Set Binding.Env.
+
+Open Scope syn.
+
+Inductive ty :=
+| Tnat : ty
+| Tarr : ty -> ty -> ty -> ty -> ty
+| Tcont : ty → ty → ty.
+
+Declare Scope types.
+
+Notation "'ℕ'" := (Tnat) : types.
+Notation "τ '∕' α '→' σ '∕' β" :=
+  (Tarr τ α σ β)
+    (at level 15
+      , σ, α, β at level 10
+      , no associativity) : types.
+Notation "τ '⤑' σ" := (Tcont τ σ) (at level 10, left associativity) : types.
+
+Reserved Notation "Γ ';' α '⊢ₑ' e ':' τ ';' β"
+  (at level 70
+    , e at level 60
+    , τ, α, β at level 20
+    , no associativity).
+
+Reserved Notation "Γ ';' α '⊢ᵥ' e ':' τ ';' β"
+  (at level 70
+    , e at level 60
+    , τ, α, β at level 20
+    , no associativity).
+
+Open Scope types.
+
+Inductive typed_expr {S : Set} (Γ : S -> ty) : ty -> expr S -> ty -> ty -> Prop :=
+| typed_Val v α τ β :
+  (Γ; α ⊢ᵥ v : τ; β) →
+  (Γ; α ⊢ₑ v : τ; β)
+| typed_Var x τ α :
+  (Γ x = τ) →
+  (Γ; α ⊢ₑ (Var x) : τ; α)
+| typed_App e₁ e₂ γ α β δ σ τ :
+  (Γ; γ ⊢ₑ e₁ : σ ∕ α → τ ∕ β; δ) →
+  (Γ; β ⊢ₑ e₂ : σ; γ) →
+  (Γ; α ⊢ₑ e₁ ⋆ e₂ : τ; δ)
+| typed_AppCont e₁ e₂ α β δ σ τ :
+  (Γ; σ ⊢ₑ e₁ : τ ⤑ α; δ) →
+  (Γ; δ ⊢ₑ e₂ : τ; β) →
+  (Γ; σ ⊢ₑ e₁ @k e₂ : α; β)
+| typed_NatOp o e₁ e₂ α β γ :
+  (Γ; α ⊢ₑ e₁ : ℕ; β) →
+  (Γ; β ⊢ₑ e₂ : ℕ; γ) →
+  (Γ; α ⊢ₑ NatOp o e₁ e₂ : ℕ; γ)
+| typed_If e e₁ e₂ α β σ τ :
+  (Γ; β ⊢ₑ e : ℕ; α) →
+  (Γ; σ ⊢ₑ e₁ : τ; β) →
+  (Γ; σ ⊢ₑ e₂ : τ; β) →
+  (Γ; σ ⊢ₑ (if e then e₁ else e₂) : τ; α)
+| typed_Shift (e : @expr (inc S)) τ α σ β :
+  (Γ ▹ τ ⤑ α; σ ⊢ₑ e : σ; β) →
+  (Γ; α ⊢ₑ shift/cc e : τ; β)
+| typed_Reset e α σ τ :
+  (Γ; σ ⊢ₑ e : σ; τ) →
+  (Γ; α ⊢ₑ reset e : τ; α)
+where "Γ ';' α '⊢ₑ' e ':' τ ';' β" := (typed_expr Γ α e τ β) : types
+with typed_val {S : Set} (Γ : S -> ty) : ty -> val S -> ty -> ty -> Prop :=
+| typed_LitV n α :
+  (Γ; α ⊢ᵥ #n : ℕ; α)
+| typed_RecV (e : expr (inc (inc S))) (δ σ τ α β : ty) :
+  (Γ ▹ (σ ∕ α → τ ∕ β) ▹ σ; α ⊢ₑ e : τ; β) ->
+  (Γ; δ ⊢ᵥ rec e : σ ∕ α → τ ∕ β; δ)
+where "Γ ';' α '⊢ᵥ' e ':' τ ';' β" := (typed_val Γ α e τ β) : types
+.
+
+Module Example.
+  Open Scope types.
+
+  Lemma typ_example1 α :
+    □; α ⊢ₑ ((#1) + (reset ((#3) + (shift/cc ((($0) @k #5) + (($0) @k #6)))))) : Tnat; α.
+  Proof.
+    econstructor.
+    - do 2 constructor.
+    - do 2 econstructor.
+      + do 2 constructor.
+      + do 2 econstructor.
+        * econstructor.
+          -- by constructor.
+          -- do 2 constructor.
+        * econstructor.
+          -- by constructor.
+          -- do 2 constructor.
+  Qed.
+
+End Example.
